end of day 15/06/18

michael_formal/EFSM_LTL.thy
@@ -11,210 +11,27 @@ definition step :: "efsm \<Rightarrow> statename \<Rightarrow> registers \<Right
 abbreviation neXt :: "efsm \<Rightarrow> statename \<Rightarrow> registers \<Rightarrow> event \<Rightarrow> ((statename \<times> outputs \<times> registers) \<Rightarrow> event \<Rightarrow> bool) \<Rightarrow> bool" where
   "neXt e s r v f \<equiv> f (step e s r (fst v) (snd v)) v"
 
-primrec globally :: "efsm \<Rightarrow> (statename \<times> outputs \<times> registers) \<Rightarrow> trace \<Rightarrow> (statename \<Rightarrow> event \<Rightarrow> registers \<Rightarrow> outputs \<Rightarrow> bool) \<Rightarrow> bool" where
-  "globally e spr [] f = f (fst spr) ('''', []) (snd (snd spr)) (fst (snd spr))" |
-  "globally e spr (h#t) f = conj (f (fst spr) h (snd (snd spr)) (fst (snd spr))) (globally e (step e (fst spr) (snd (snd spr)) (fst h) (snd h)) t f)"
+primrec globally :: "efsm \<Rightarrow> (statename \<times> outputs \<times> registers) \<Rightarrow> trace \<Rightarrow> ((statename \<times> outputs \<times> registers) \<Rightarrow> event \<Rightarrow> bool) \<Rightarrow> bool" where
+  "globally e spr [] f = f spr ('''', [])" |
+  "globally e spr (h#t) f = conj (f spr h) (globally e (step e (fst spr) (snd (snd spr)) (fst h) (snd h)) t f)"
 
-lemma read_not_none : "\<forall>r'. step filesystem 2 r ''read'' [] \<noteq> (0, [], r')"
-  by (simp add: fs_simp step_def)
-
-lemma read_no_side_effects : "\<exists>p. step filesystem 2 r ''read'' [] = (2, p, r)"
-  apply (simp add: fs_simp step_def)
-  apply (case_tac "r ''r1'' = r ''r3''")
-   apply simp
-  apply (rule ext)
-  by auto
-
-lemma read_no_side_effects2 : "step filesystem 2 r ''read'' [] = a \<Longrightarrow> snd (snd a) = r \<and> fst a = 2"
-  apply (simp add: step_def)
-  apply (simp add: fs_simp)
-  apply (case_tac "r ''r1'' = r ''r3''")
-   apply simp
-   apply safe[1]
-    apply (rule ext, simp, simp)
+lemma "globally filesystem (s,outs,r) t (\<lambda>(s, p, r) e. s \<noteq> 0) \<longrightarrow>
+globally filesystem (s,outs,r) t (\<lambda>(s, p, r) e. (fst e = ''write'' \<and> r ''r1'' = 0 \<and> snd e \<noteq> [0]) \<longrightarrow>
+  globally filesystem (s, p, r) t (\<lambda>(s', p', r') e'. (s' = 2 \<and> fst e' = ''read'' \<and> r' ''r1'' \<noteq> 0)\<longrightarrow>
+    (fst (snd (step filesystem s' r' (fst e') (snd e')))) = [0]))"
   apply simp
-  apply safe
-  by (rule ext, simp, simp)
-
-lemma truefun : "\<forall> e spr. globally e spr t (\<lambda>s e r' p. True)"
-proof (induction t)
-  case Nil
-  then show ?case by simp
-next
-  case (Cons a t)
-  then show ?case
-    apply simp
-    by (simp add: Cons.IH)
-qed
-
-lemma read_denied: "r ''r1'' \<noteq> 1 \<Longrightarrow> r ''r3'' = 1 \<Longrightarrow> EFSM_LTL.step filesystem 2 r ''read'' [] = (2, [0], r)"
-  apply (simp add: fs_simp step_def)
-  by (rule ext, simp)
-
-lemma read_success: "r ''r1''= r ''r3'' \<Longrightarrow> EFSM_LTL.step filesystem 2 r ''read'' [] = (2, [r ''r2''], r)"
-  apply (simp add: fs_simp step_def)
-  by (rule ext, simp)
-
-lemma read_denied1: "r ''r1'' \<noteq> r ''r3'' \<Longrightarrow> EFSM_LTL.step filesystem 2 r ''read'' [] = (2, [0], r)"
-  apply (simp add: fs_simp step_def)
-  by (rule ext, simp)
-
-lemma read_step: "step filesystem 2 r ''read'' [] = (2, [r ''r2''], r) \<or> step filesystem 2 r ''read'' [] = (2, [0], r)"
-  apply (case_tac "r ''r1'' = r ''r3''")
-   apply (simp add: read_success)
-  by (simp add: read_denied1)
-
-lemma logout: "(EFSM_LTL.step filesystem 2 r ''logout'' []) = (1, [], r)"
-  apply (simp add: fs_simp step_def)
-  by (rule ext, simp)
-
-lemma login_2: "fst a = ''login'' \<Longrightarrow> EFSM_LTL.step filesystem 2 r (fst a) (snd a) = (0, [], r)"
-  by (simp add: fs_simp step_def)
-
-lemma index2state_i1: "length (snd a) = Suc 0 \<Longrightarrow> index2state (snd a) 1 ''i1'' = hd (snd a)"
-  by (metis Suc_length_conv i1 index2state.simps(2) list.sel(1))
-
-lemma writes: "fst a = ''write'' \<and> length (snd a) = Suc 0 \<Longrightarrow>
-                r ''r1'' \<noteq> r ''r3'' \<Longrightarrow> 
-                EFSM_LTL.step filesystem 2 r ''write'' (snd a) = (2, [], (\<lambda>x. if x = ''r2'' then hd (snd a) else (if x = ''r3'' then r ''r1'' else r x)))"
-  apply (simp add: fs_simp step_def)
-  apply safe
-  apply (rule ext)
-  apply simp
-  by (simp add: index2state_i1)
-
-lemma nomoreinputs: "a \<noteq> (''read'', []) \<Longrightarrow>
-         a \<noteq> (''logout'', []) \<Longrightarrow>
-         fst a \<noteq> ''write'' \<Longrightarrow>
-         (EFSM_LTL.step filesystem 2 r (fst a) (snd a)) = (0, [],r)"
-  apply (simp add: fs_simp step_def)
-  by (metis prod.collapse)
-
-lemma dead_state: "globally filesystem (0, [], r) t (\<lambda>s e r' p. s \<noteq> 0) \<Longrightarrow> False"
 proof (induction t)
 case Nil
-  then show ?case by simp
+then show ?case by simp
 next
   case (Cons a t)
-  then show ?case by simp
-qed
-
-lemma login_1: "fst a = ''login'' \<and> length (snd a) = Suc 0 \<Longrightarrow> step filesystem 1 r ''login'' (snd a) = (2, [], (\<lambda>x. if x = ''r1'' then hd (snd a) else r x))"
-  apply (simp add: fs_simp step_def)
-  apply (rule ext)
-  by (simp add: index2state_i1)
-
-lemma login_user_1: "EFSM_LTL.step filesystem 1 reg ''login'' [1] = (2, [], (\<lambda>x. if x = ''r1'' then 1 else reg x))"
-  apply (simp add: fs_simp step_def)
-  apply (rule ext)
-  by simp
-
-(*
-noChangeOwner: THEOREM filesystem |- FORALL (user : UID): 
-G(cfstate /= NULL_STATE) => 
-G( 
-  (label=write AND r_1=user AND ip_1_write_1/=accessDenied) => 
-  G((cfstate=S_2 AND label=read AND r_1/=user) => 
-    X(op_1_read_0 = accessDenied) 
-  ) 
-  );
-*)
-
-lemma "globally filesystem (state, outs, r) t (\<lambda>s e r p. s \<noteq> 0) \<longrightarrow>
-globally filesystem (state, outs, reg) t (\<lambda>s e r p. (fst e = ''write'' \<and> r ''r1'' = 1 \<and> snd e \<noteq> [0]) \<longrightarrow>
-  globally filesystem (state, outs, reg) t (\<lambda>s' e' r' p'. (s' = 2 \<and> fst e' = ''read'' \<and> r' ''r1'' \<noteq> 1)\<longrightarrow>
-    (fst (snd (step filesystem s' r' (fst e') (snd e')))) = [0])
-)"
-proof (induction t)
-  case Nil
-  then show ?case by simp
-next
-  case (Cons a t')
   then show ?case
     apply simp
-    apply (case_tac "state = 0") (* If we're in state zero, it doesn't matter *)
-     apply (simp)
-    apply (case_tac "state = 1") (* If we were in state 1 to start with and prepend something *)
+    apply (case_tac "s = 0")
      apply simp
-     apply (case_tac "fst a = ''login'' \<and> length (snd a) = 1")
+    apply (case_tac "s = 1")
     apply simp
-
 qed
 
-lemma "\<forall> outs. globally filesystem (state, outs, r) t (\<lambda>s e r p. s \<noteq> 0) \<longrightarrow>
-globally filesystem (state, outs, r) t (\<lambda>s e r p. (fst e = ''write'' \<and> r' ''r1'' = 1 \<and> snd e \<noteq> [0]) \<longrightarrow>
-  globally filesystem (state, outs, r) t (\<lambda>s e r p. (s = 2 \<and> fst e = ''read'' \<and> r' ''r1'' \<noteq> 1)) \<longrightarrow>
-    neXt filesystem state r (hd t) (\<lambda>spr e. (fst (snd spr)) = [0])
-)"
-proof (induction t)
-  case Nil
-  then show ?case by simp
-next
-  case (Cons a t')
-  then show ?case
-    apply simp
-    apply (case_tac "state = 0", simp)
-    apply (case_tac "state = 1", simp)
-     apply (case_tac "fst a = ''login'' \<and> length (snd a) = 1")
-      apply (simp add: truefun)
-     apply (simp add: truefun)
-    apply (case_tac "state = 2", simp)
-     apply (simp add: truefun)
-    by (simp add: truefun)
-qed
 
-lemma "all (t) (\<lambda>e. e = (''read'', []) \<or> e = (''login'', []) \<or> e = (''logout'', []) \<or> (fst e = ''write'' \<and> length (snd e) = 1)) \<Longrightarrow>
- \<forall> outs r. globally filesystem (state, outs, r) t (\<lambda>s e r' p. s \<noteq> 0) \<longrightarrow>
-globally filesystem (state, outs, r) t (\<lambda>s e r' p. (s = 2 \<and> fst e = ''write'' \<and> r' ''r1'' = 1) \<longrightarrow>
-  globally filesystem (state, outs, r) t (\<lambda>s e r' p. (s = 2 \<and> fst e = ''read'' \<and> r' ''r1'' \<noteq> 1)) \<longrightarrow>
-    neXt filesystem s' r'' (hd t') (\<lambda>spr e. (fst (snd spr)) = [0])
-)"
-proof (induction t)
-  case Nil
-  then show ?case by simp
-next
-  case (Cons a t')
-  then show ?case
-    apply (case_tac "state = 2")
-     apply (case_tac "a = (''read'', [])", simp)
-      apply (rule allI)
-      apply (case_tac "(EFSM_LTL.step filesystem 2 r ''read'' []) = (2, [0], r)", simp)
-       apply (case_tac "r ''r1'' = 1")
-        apply (simp add: truefun)
-       apply simp
-      apply (case_tac "r ''r1'' = 1")
-       apply (simp add: truefun)
-      apply simp
-      apply (case_tac "r ''r3'' = 1")
-       apply (simp add: read_denied)
-      apply (case_tac "r ''r1'' = r ''r3''")
-       apply (simp add: read_success)
-      apply (simp add: read_denied1)
-
-     apply (case_tac "fst a = ''write'' \<and> length (snd a) = 1", simp)
-      apply (frule allI)
-      apply (case_tac "r ''r1'' = r ''r3''")
-    using truefun apply blast
-      apply (simp add: writes truefun)
-
-    apply (case_tac "a = (''logout'', [])", simp)
-    apply (simp add: logout truefun)
-
-     apply (rule allI, rule allI)
-     apply safe
-      apply (simp add: nomoreinputs)
-      apply (metis (no_types, lifting) dead_state fst_conv login_2)
-
-     apply simp
-     apply (metis (no_types, lifting) dead_state fst_conv login_2)
-
-    apply (case_tac "state = 0")
-     apply simp
-
-    apply (case_tac "state = 1")
-     apply (case_tac "fst a = ''login'' \<and> length (snd a) = 1")
-      apply (simp add: truefun)
-     apply (simp add: truefun)
-    by (simp add: truefun)
-qed
 end
